src/Std/Tactic/BVDecide/LRAT/Internal/Convert.lean
@@ -132,18 +132,22 @@ theorem CNF.unsat_of_convertLRAT_unsat (cnf : CNF Nat) :
   apply h1
   simp only [Formula.formulaEntails_def, List.all_eq_true, decide_eq_true_eq]
   intro lratClause hlclause
-  simp only [Formula.toList, DefaultFormula.toList, DefaultFormula.ofArray,
-    CNF.convertLRAT', List.size_toArray, List.toList_toArray,
-    List.map_nil, List.append_nil, List.mem_filterMap, id_eq, exists_eq_right] at hlclause
-  sorry
-  --rcases hlclause with ⟨reflectClause, ⟨hrclause1, hrclause2⟩⟩
-  --simp only [CNF.eval, List.all_eq_true] at h2
-  --split at hrclause2
-  --next heq =>
-  --  rw [← heq] at hrclause2
-  --  simp only [Option.some.injEq] at hrclause2
-  --  simp [CNF.Clause.convertLRAT_sat_of_sat reflectClause hrclause2, h2 reflectClause hrclause1]
-  --· contradiction
+  simp only [Formula.toList, DefaultFormula.toList, DefaultFormula.ofArray, convertLRAT',
+    Array.size_append, List.size_toArray, List.length_cons, List.length_nil, Nat.zero_add,
+    Array.foldl_append', List.foldl_toArray', List.foldl_cons,
+    List.foldl_nil, Array.toList_append, Array.toList_filterMap', List.cons_append, List.nil_append,
+    List.toList_toArray, id_eq, List.filterMap_cons_none, List.map_nil, List.append_nil,
+    List.mem_filterMap, Array.mem_toList_iff, exists_eq_right] at hlclause
+  rcases hlclause with ⟨reflectClause, ⟨hrclause1, hrclause2⟩⟩
+  simp only [CNF.eval, Array.all_eq_true] at h2
+  split at hrclause2
+  · next heq =>
+    rw [← heq] at hrclause2
+    simp only [Option.some.injEq] at hrclause2
+    rw [Array.mem_iff_getElem] at hrclause1
+    rcases hrclause1 with ⟨i, h, rfl⟩
+    simp [CNF.Clause.convertLRAT_sat_of_sat _ hrclause2, h2 i h]
+  · contradiction
 
 end Internal
 end LRAT
